src/cbor/pulse/raw/everparse/CBOR.Pulse.Raw.EverParse.Det.Impl.fst
@@ -844,10 +844,10 @@ fn cbor_det_array_iterator_share (_: unit) : share_t cbor_det_array_iterator_mat
   unfold (I.iterator_match RawMatch.cbor_raw_match SpecRawEverParse.parse_raw_data_item pm it
     (Ghost.reveal lr));
   with l1 l2 . assert (
-    I.base_mixed_list_match RawMatch.cbor_raw_match SpecRawEverParse.parse_raw_data_item pm it.LowParse.PulseParse.Iterator.Type.before l1 **
-    I.mixed_list_match RawMatch.cbor_raw_match SpecRawEverParse.parse_raw_data_item pm it.LowParse.PulseParse.Iterator.Type.after l2);
-  I.base_mixed_list_match_share RawMatch.cbor_raw_match SpecRawEverParse.parse_raw_data_item pm it.LowParse.PulseParse.Iterator.Type.before l1 cbor_raw_match_share_aux;
-  I.mixed_list_match_share RawMatch.cbor_raw_match SpecRawEverParse.parse_raw_data_item pm it.LowParse.PulseParse.Iterator.Type.after l2 cbor_raw_match_share_aux;
+    I.base_mixed_list_match RawMatch.cbor_raw_match SpecRawEverParse.parse_raw_data_item pm (IT.iter_before it) l1 **
+    I.mixed_list_match RawMatch.cbor_raw_match SpecRawEverParse.parse_raw_data_item pm (IT.iter_after it) l2);
+  I.base_mixed_list_match_share RawMatch.cbor_raw_match SpecRawEverParse.parse_raw_data_item pm (IT.iter_before it) l1 cbor_raw_match_share_aux;
+  I.mixed_list_match_share RawMatch.cbor_raw_match SpecRawEverParse.parse_raw_data_item pm (IT.iter_after it) l2 cbor_raw_match_share_aux;
   fold (I.iterator_match RawMatch.cbor_raw_match SpecRawEverParse.parse_raw_data_item (pm /. 2.0R) it
     (Ghost.reveal lr));
   fold (I.iterator_match RawMatch.cbor_raw_match SpecRawEverParse.parse_raw_data_item (pm /. 2.0R) it
@@ -879,13 +879,13 @@ fn cbor_det_array_iterator_gather (_: unit) : gather_t cbor_det_array_iterator_m
   unfold (I.iterator_match RawMatch.cbor_raw_match SpecRawEverParse.parse_raw_data_item pm it (Ghost.reveal lr));
   unfold (I.iterator_match RawMatch.cbor_raw_match SpecRawEverParse.parse_raw_data_item pm' it (Ghost.reveal lr'));
   with l1 l2 . assert (
-    I.base_mixed_list_match RawMatch.cbor_raw_match SpecRawEverParse.parse_raw_data_item pm it.LowParse.PulseParse.Iterator.Type.before l1 **
-    I.mixed_list_match RawMatch.cbor_raw_match SpecRawEverParse.parse_raw_data_item pm it.LowParse.PulseParse.Iterator.Type.after l2);
+    I.base_mixed_list_match RawMatch.cbor_raw_match SpecRawEverParse.parse_raw_data_item pm (IT.iter_before it) l1 **
+    I.mixed_list_match RawMatch.cbor_raw_match SpecRawEverParse.parse_raw_data_item pm (IT.iter_after it) l2);
   with l1' l2' . assert (
-    I.base_mixed_list_match RawMatch.cbor_raw_match SpecRawEverParse.parse_raw_data_item pm' it.LowParse.PulseParse.Iterator.Type.before l1' **
-    I.mixed_list_match RawMatch.cbor_raw_match SpecRawEverParse.parse_raw_data_item pm' it.LowParse.PulseParse.Iterator.Type.after l2');
-  I.base_mixed_list_match_gather RawMatch.cbor_raw_match SpecRawEverParse.parse_raw_data_item pm pm' it.LowParse.PulseParse.Iterator.Type.before l1 l1' cbor_raw_match_gather_aux;
-  I.mixed_list_match_gather RawMatch.cbor_raw_match SpecRawEverParse.parse_raw_data_item pm pm' it.LowParse.PulseParse.Iterator.Type.after l2 l2' cbor_raw_match_gather_aux;
+    I.base_mixed_list_match RawMatch.cbor_raw_match SpecRawEverParse.parse_raw_data_item pm' (IT.iter_before it) l1' **
+    I.mixed_list_match RawMatch.cbor_raw_match SpecRawEverParse.parse_raw_data_item pm' (IT.iter_after it) l2');
+  I.base_mixed_list_match_gather RawMatch.cbor_raw_match SpecRawEverParse.parse_raw_data_item pm pm' (IT.iter_before it) l1 l1' cbor_raw_match_gather_aux;
+  I.mixed_list_match_gather RawMatch.cbor_raw_match SpecRawEverParse.parse_raw_data_item pm pm' (IT.iter_after it) l2 l2' cbor_raw_match_gather_aux;
   List.Tot.append_injective l1 l1' l2 l2';
   fold (I.iterator_match RawMatch.cbor_raw_match SpecRawEverParse.parse_raw_data_item (pm +. pm') it (Ghost.reveal lr));
   rewrite (I.iterator_match RawMatch.cbor_raw_match SpecRawEverParse.parse_raw_data_item (pm +. pm') it (Ghost.reveal lr))
@@ -904,11 +904,11 @@ fn cbor_det_array_iterator_is_empty (_: unit) : array_iterator_is_empty_t cbor_d
        as (I.iterator_match RawMatch.cbor_raw_match SpecRawEverParse.parse_raw_data_item p x (Ghost.reveal lr));
   unfold (I.iterator_match RawMatch.cbor_raw_match SpecRawEverParse.parse_raw_data_item p x (Ghost.reveal lr));
   with l1 l2 . assert (
-    I.base_mixed_list_match RawMatch.cbor_raw_match SpecRawEverParse.parse_raw_data_item p x.LowParse.PulseParse.Iterator.Type.before l1 **
-    I.mixed_list_match RawMatch.cbor_raw_match SpecRawEverParse.parse_raw_data_item p x.LowParse.PulseParse.Iterator.Type.after l2);
-  I.base_mixed_list_match_length RawMatch.cbor_raw_match SpecRawEverParse.parse_raw_data_item p x.LowParse.PulseParse.Iterator.Type.before l1;
-  I.mixed_list_match_length RawMatch.cbor_raw_match SpecRawEverParse.parse_raw_data_item p x.LowParse.PulseParse.Iterator.Type.after l2;
-  let len_before = IT.base_mixed_list_length x.LowParse.PulseParse.Iterator.Type.before;
+    I.base_mixed_list_match RawMatch.cbor_raw_match SpecRawEverParse.parse_raw_data_item p (IT.iter_before x) l1 **
+    I.mixed_list_match RawMatch.cbor_raw_match SpecRawEverParse.parse_raw_data_item p (IT.iter_after x) l2);
+  I.base_mixed_list_match_length RawMatch.cbor_raw_match SpecRawEverParse.parse_raw_data_item p (IT.iter_before x) l1;
+  I.mixed_list_match_length RawMatch.cbor_raw_match SpecRawEverParse.parse_raw_data_item p (IT.iter_after x) l2;
+  let len_before = IT.base_mixed_list_length (IT.iter_before x);
   Aux.length_det_raw_list y;
   let res = (len_before = 0sz);
   fold (I.iterator_match RawMatch.cbor_raw_match SpecRawEverParse.parse_raw_data_item p x (Ghost.reveal lr));
@@ -998,13 +998,13 @@ fn cbor_det_array_iterator_length (_: unit) : array_iterator_length_t cbor_det_a
        as (I.iterator_match RawMatch.cbor_raw_match SpecRawEverParse.parse_raw_data_item p x (Ghost.reveal lr));
   unfold (I.iterator_match RawMatch.cbor_raw_match SpecRawEverParse.parse_raw_data_item p x (Ghost.reveal lr));
   with l1 l2 . assert (
-    I.base_mixed_list_match RawMatch.cbor_raw_match SpecRawEverParse.parse_raw_data_item p x.LowParse.PulseParse.Iterator.Type.before l1 **
-    I.mixed_list_match RawMatch.cbor_raw_match SpecRawEverParse.parse_raw_data_item p x.LowParse.PulseParse.Iterator.Type.after l2);
-  I.base_mixed_list_match_length RawMatch.cbor_raw_match SpecRawEverParse.parse_raw_data_item p x.LowParse.PulseParse.Iterator.Type.before l1;
-  I.mixed_list_match_length RawMatch.cbor_raw_match SpecRawEverParse.parse_raw_data_item p x.LowParse.PulseParse.Iterator.Type.after l2;
+    I.base_mixed_list_match RawMatch.cbor_raw_match SpecRawEverParse.parse_raw_data_item p (IT.iter_before x) l1 **
+    I.mixed_list_match RawMatch.cbor_raw_match SpecRawEverParse.parse_raw_data_item p (IT.iter_after x) l2);
+  I.base_mixed_list_match_length RawMatch.cbor_raw_match SpecRawEverParse.parse_raw_data_item p (IT.iter_before x) l1;
+  I.mixed_list_match_length RawMatch.cbor_raw_match SpecRawEverParse.parse_raw_data_item p (IT.iter_after x) l2;
   Aux.length_det_raw_list y;
-  let len_before = IT.base_mixed_list_length x.LowParse.PulseParse.Iterator.Type.before;
-  let len_after = IT.mixed_list_length x.LowParse.PulseParse.Iterator.Type.after;
+  let len_before = IT.base_mixed_list_length (IT.iter_before x);
+  let len_after = IT.mixed_list_length (IT.iter_after x);
   List.Tot.append_length l1 l2;
   SZ.fits_u64_implies_fits (SZ.v len_before + SZ.v len_after);
   let len_total = SZ.add len_before len_after;
@@ -1163,33 +1163,33 @@ fn cbor_det_array_iterator_truncate (_: unit) : array_iterator_truncate_t cbor_d
        as (I.iterator_match RawMatch.cbor_raw_match SpecRawEverParse.parse_raw_data_item py x (Ghost.reveal lr));
   unfold (I.iterator_match RawMatch.cbor_raw_match SpecRawEverParse.parse_raw_data_item py x (Ghost.reveal lr));
   with l1 l2 . assert (
-    I.base_mixed_list_match RawMatch.cbor_raw_match SpecRawEverParse.parse_raw_data_item py x.LowParse.PulseParse.Iterator.Type.before l1 **
-    I.mixed_list_match RawMatch.cbor_raw_match SpecRawEverParse.parse_raw_data_item py x.LowParse.PulseParse.Iterator.Type.after l2);
-  I.base_mixed_list_match_length RawMatch.cbor_raw_match SpecRawEverParse.parse_raw_data_item py x.LowParse.PulseParse.Iterator.Type.before l1;
-  I.mixed_list_match_length RawMatch.cbor_raw_match SpecRawEverParse.parse_raw_data_item py x.LowParse.PulseParse.Iterator.Type.after l2;
+    I.base_mixed_list_match RawMatch.cbor_raw_match SpecRawEverParse.parse_raw_data_item py (IT.iter_before x) l1 **
+    I.mixed_list_match RawMatch.cbor_raw_match SpecRawEverParse.parse_raw_data_item py (IT.iter_after x) l2);
+  I.base_mixed_list_match_length RawMatch.cbor_raw_match SpecRawEverParse.parse_raw_data_item py (IT.iter_before x) l1;
+  I.mixed_list_match_length RawMatch.cbor_raw_match SpecRawEverParse.parse_raw_data_item py (IT.iter_after x) l2;
   Aux.length_det_raw_list z;
-  let cb_sz = IT.base_mixed_list_length x.LowParse.PulseParse.Iterator.Type.before;
+  let cb_sz = IT.base_mixed_list_length (IT.iter_before x);
   let len_before_sz = (if SZ.lte len_sz cb_sz then len_sz else cb_sz);
   let len_after_sz = (if SZ.lte len_sz cb_sz then 0sz else SZ.sub len_sz cb_sz);
   // Narrow before to first len_before_sz elements
-  rewrite (I.base_mixed_list_match RawMatch.cbor_raw_match SpecRawEverParse.parse_raw_data_item py x.LowParse.PulseParse.Iterator.Type.before l1)
-       as (I.base_mixed_list_match_n RawMatch.cbor_raw_match SpecRawEverParse.parse_raw_data_item 0 (SZ.v cb_sz) py x.LowParse.PulseParse.Iterator.Type.before l1);
+  rewrite (I.base_mixed_list_match RawMatch.cbor_raw_match SpecRawEverParse.parse_raw_data_item py (IT.iter_before x) l1)
+       as (I.base_mixed_list_match_n RawMatch.cbor_raw_match SpecRawEverParse.parse_raw_data_item 0 (SZ.v cb_sz) py (IT.iter_before x) l1);
   let bi' = I.base_mixed_list_narrow_n
     RawMatch.cbor_raw_match SpecRawEverParse.parse_raw_data_item
-    Validate.jump_raw_data_item_eta 0 (SZ.v cb_sz) py x.LowParse.PulseParse.Iterator.Type.before l1
+    Validate.jump_raw_data_item_eta 0 (SZ.v cb_sz) py (IT.iter_before x) l1
     0sz len_before_sz;
   // bi' : base_mixed_list cbor_raw with base_mixed_list_match bi' (list_narrow l1 0 (SZ.v len_before_sz)) at pm
   // plus trade (...) (base_mixed_list_match_n before)
   // Narrow after to first len_after_sz elements
-  let ca_sz = IT.mixed_list_length x.LowParse.PulseParse.Iterator.Type.after;
+  let ca_sz = IT.mixed_list_length (IT.iter_after x);
   // Re-establish bounds: U64.v len <= List.Tot.length z = SZ.v cb_sz + SZ.v ca_sz
   List.Tot.append_length l1 l2;
   assert (pure (SZ.v len_after_sz <= SZ.v ca_sz));
-  rewrite (I.mixed_list_match RawMatch.cbor_raw_match SpecRawEverParse.parse_raw_data_item py x.LowParse.PulseParse.Iterator.Type.after l2)
-       as (I.mixed_list_match_n RawMatch.cbor_raw_match SpecRawEverParse.parse_raw_data_item 0 (SZ.v ca_sz) py x.LowParse.PulseParse.Iterator.Type.after l2);
+  rewrite (I.mixed_list_match RawMatch.cbor_raw_match SpecRawEverParse.parse_raw_data_item py (IT.iter_after x) l2)
+       as (I.mixed_list_match_n RawMatch.cbor_raw_match SpecRawEverParse.parse_raw_data_item 0 (SZ.v ca_sz) py (IT.iter_after x) l2);
   let after' = I.mixed_list_narrow_n
     RawMatch.cbor_raw_match SpecRawEverParse.parse_raw_data_item
-    Validate.jump_raw_data_item_eta 0 (SZ.v ca_sz) py x.LowParse.PulseParse.Iterator.Type.after l2
+    Validate.jump_raw_data_item_eta 0 (SZ.v ca_sz) py (IT.iter_after x) l2
     0sz len_after_sz
     cbor_raw_match_share_aux cbor_raw_match_gather_aux;
   // after' : mixed_list cbor_raw with mixed_list_match after' (list_narrow l2 0 (SZ.v len_after_sz)) at pm/2
@@ -1213,7 +1213,7 @@ fn cbor_det_array_iterator_truncate (_: unit) : array_iterator_truncate_t cbor_d
   // Rewrite the second copy of base_mixed_list_match_n to use l1_narrow form
   rewrite each (LowParse.PulseParse.Iterator.list_narrow l1 0 (SZ.v len_before_sz)) as (Ghost.reveal l1_narrow);
   rewrite each (LowParse.PulseParse.Iterator.list_narrow l2 0 (SZ.v len_after_sz)) as (Ghost.reveal l2_narrow);
-  let it' : LowParse.PulseParse.Iterator.Type.iterator RawType.cbor_raw = { before = bi'; after = after' };
+  let it' : LowParse.PulseParse.Iterator.Type.iterator RawType.cbor_raw = IT.IPair bi' after';
   // Establish the truncated list relation
   // take n (l1 ++ l2) == l1_narrow ++ l2_narrow
   List.Tot.append_length l1 l2;
@@ -1230,9 +1230,9 @@ fn cbor_det_array_iterator_truncate (_: unit) : array_iterator_truncate_t cbor_d
   assert (pure (Aux.det_raw_list z_take == LowParse.PulseParse.Iterator.list_narrow (Ghost.reveal lr) 0 (Ghost.reveal n)));
   // Rewrite the matches (l1_narrow ghost was already substituted by rewrite each above)
   rewrite (I.base_mixed_list_match RawMatch.cbor_raw_match SpecRawEverParse.parse_raw_data_item (py /. 2.0R) bi' (Ghost.reveal l1_narrow))
-       as (I.base_mixed_list_match RawMatch.cbor_raw_match SpecRawEverParse.parse_raw_data_item (py /. 2.0R) it'.LowParse.PulseParse.Iterator.Type.before (Ghost.reveal l1_narrow));
+       as (I.base_mixed_list_match RawMatch.cbor_raw_match SpecRawEverParse.parse_raw_data_item (py /. 2.0R) (IT.iter_before it') (Ghost.reveal l1_narrow));
   rewrite (I.mixed_list_match RawMatch.cbor_raw_match SpecRawEverParse.parse_raw_data_item (py /. 2.0R) after' (Ghost.reveal l2_narrow))
-       as (I.mixed_list_match RawMatch.cbor_raw_match SpecRawEverParse.parse_raw_data_item (py /. 2.0R) it'.LowParse.PulseParse.Iterator.Type.after (Ghost.reveal l2_narrow));
+       as (I.mixed_list_match RawMatch.cbor_raw_match SpecRawEverParse.parse_raw_data_item (py /. 2.0R) (IT.iter_after it') (Ghost.reveal l2_narrow));
   fold (I.iterator_match RawMatch.cbor_raw_match SpecRawEverParse.parse_raw_data_item (py /. 2.0R) it' (Aux.det_raw_list z_take));
   fold (cbor_det_array_iterator_match (py /. 2.0R) it' z_take);
   // Construct the trade back. The "extra" carries:
@@ -1245,10 +1245,10 @@ fn cbor_det_array_iterator_truncate (_: unit) : array_iterator_truncate_t cbor_d
     (I.base_mixed_list_match_n RawMatch.cbor_raw_match SpecRawEverParse.parse_raw_data_item 0 (SZ.v len_before_sz) (py /. 2.0R) bi' (Ghost.reveal l1_narrow) **
      Trade.trade
        (I.base_mixed_list_match RawMatch.cbor_raw_match SpecRawEverParse.parse_raw_data_item py bi' (Ghost.reveal l1_narrow))
-       (I.base_mixed_list_match_n RawMatch.cbor_raw_match SpecRawEverParse.parse_raw_data_item 0 (SZ.v cb_sz) py x.LowParse.PulseParse.Iterator.Type.before l1) **
+       (I.base_mixed_list_match_n RawMatch.cbor_raw_match SpecRawEverParse.parse_raw_data_item 0 (SZ.v cb_sz) py (IT.iter_before x) l1) **
      Trade.trade
        (I.mixed_list_match RawMatch.cbor_raw_match SpecRawEverParse.parse_raw_data_item (py /. 2.0R) after' (Ghost.reveal l2_narrow))
-       (I.mixed_list_match_n RawMatch.cbor_raw_match SpecRawEverParse.parse_raw_data_item 0 (SZ.v ca_sz) py x.LowParse.PulseParse.Iterator.Type.after l2))
+       (I.mixed_list_match_n RawMatch.cbor_raw_match SpecRawEverParse.parse_raw_data_item 0 (SZ.v ca_sz) py (IT.iter_after x) l2))
     fn _ {
       // Body: given cbor_det_array_iterator_match it' z_take, recover orig
       unfold (cbor_det_array_iterator_match (py /. 2.0R) it' z_take);
@@ -1256,20 +1256,20 @@ fn cbor_det_array_iterator_truncate (_: unit) : array_iterator_truncate_t cbor_d
            as (I.iterator_match RawMatch.cbor_raw_match SpecRawEverParse.parse_raw_data_item (py /. 2.0R) it' (List.Tot.append (Ghost.reveal l1_narrow) (Ghost.reveal l2_narrow)));
       unfold (I.iterator_match RawMatch.cbor_raw_match SpecRawEverParse.parse_raw_data_item (py /. 2.0R) it' (List.Tot.append (Ghost.reveal l1_narrow) (Ghost.reveal l2_narrow)));
       with xl1 xl2 . assert (
-        I.base_mixed_list_match RawMatch.cbor_raw_match SpecRawEverParse.parse_raw_data_item (py /. 2.0R) it'.LowParse.PulseParse.Iterator.Type.before xl1 **
-        I.mixed_list_match RawMatch.cbor_raw_match SpecRawEverParse.parse_raw_data_item (py /. 2.0R) it'.LowParse.PulseParse.Iterator.Type.after xl2);
+        I.base_mixed_list_match RawMatch.cbor_raw_match SpecRawEverParse.parse_raw_data_item (py /. 2.0R) (IT.iter_before it') xl1 **
+        I.mixed_list_match RawMatch.cbor_raw_match SpecRawEverParse.parse_raw_data_item (py /. 2.0R) (IT.iter_after it') xl2);
       // The split is uniquely determined: xl1 has length len_before_sz (from base_mixed_list_match_length on bi'), xl2 has length len_after_sz.
-      I.base_mixed_list_match_length RawMatch.cbor_raw_match SpecRawEverParse.parse_raw_data_item (py /. 2.0R) it'.LowParse.PulseParse.Iterator.Type.before xl1;
-      I.mixed_list_match_length RawMatch.cbor_raw_match SpecRawEverParse.parse_raw_data_item (py /. 2.0R) it'.LowParse.PulseParse.Iterator.Type.after xl2;
+      I.base_mixed_list_match_length RawMatch.cbor_raw_match SpecRawEverParse.parse_raw_data_item (py /. 2.0R) (IT.iter_before it') xl1;
+      I.mixed_list_match_length RawMatch.cbor_raw_match SpecRawEverParse.parse_raw_data_item (py /. 2.0R) (IT.iter_after it') xl2;
       // From xl1++xl2 == l1_narrow++l2_narrow with len(xl1)==len(l1_narrow), conclude xl1==l1_narrow and xl2==l2_narrow
       List.Tot.append_length (Ghost.reveal l1_narrow) (Ghost.reveal l2_narrow);
       List.Tot.append_length xl1 xl2;
       List.Tot.append_injective xl1 (Ghost.reveal l1_narrow) xl2 (Ghost.reveal l2_narrow);
       rewrite each xl1 as (Ghost.reveal l1_narrow);
       rewrite each xl2 as (Ghost.reveal l2_narrow);
-      rewrite (I.base_mixed_list_match RawMatch.cbor_raw_match SpecRawEverParse.parse_raw_data_item (py /. 2.0R) it'.LowParse.PulseParse.Iterator.Type.before (Ghost.reveal l1_narrow))
+      rewrite (I.base_mixed_list_match RawMatch.cbor_raw_match SpecRawEverParse.parse_raw_data_item (py /. 2.0R) (IT.iter_before it') (Ghost.reveal l1_narrow))
            as (I.base_mixed_list_match RawMatch.cbor_raw_match SpecRawEverParse.parse_raw_data_item (py /. 2.0R) bi' (Ghost.reveal l1_narrow));
-      rewrite (I.mixed_list_match RawMatch.cbor_raw_match SpecRawEverParse.parse_raw_data_item (py /. 2.0R) it'.LowParse.PulseParse.Iterator.Type.after (Ghost.reveal l2_narrow))
+      rewrite (I.mixed_list_match RawMatch.cbor_raw_match SpecRawEverParse.parse_raw_data_item (py /. 2.0R) (IT.iter_after it') (Ghost.reveal l2_narrow))
            as (I.mixed_list_match RawMatch.cbor_raw_match SpecRawEverParse.parse_raw_data_item (py /. 2.0R) after' (Ghost.reveal l2_narrow));
       // Gather two pm/2 copies of bi' to pm
       rewrite (I.base_mixed_list_match RawMatch.cbor_raw_match SpecRawEverParse.parse_raw_data_item (py /. 2.0R) bi' (Ghost.reveal l1_narrow))
@@ -1279,14 +1279,14 @@ fn cbor_det_array_iterator_truncate (_: unit) : array_iterator_truncate_t cbor_d
       rewrite (I.base_mixed_list_match_n RawMatch.cbor_raw_match SpecRawEverParse.parse_raw_data_item 0 (SZ.v len_before_sz) (py /. 2.0R +. py /. 2.0R) bi' (Ghost.reveal l1_narrow))
            as (I.base_mixed_list_match RawMatch.cbor_raw_match SpecRawEverParse.parse_raw_data_item py bi' (Ghost.reveal l1_narrow));
       // Use trade narrow_before to recover the original before
-      Trade.elim _ (I.base_mixed_list_match_n RawMatch.cbor_raw_match SpecRawEverParse.parse_raw_data_item 0 (SZ.v cb_sz) py x.LowParse.PulseParse.Iterator.Type.before l1);
+      Trade.elim _ (I.base_mixed_list_match_n RawMatch.cbor_raw_match SpecRawEverParse.parse_raw_data_item 0 (SZ.v cb_sz) py (IT.iter_before x) l1);
       // Use trade narrow_after on after'
-      Trade.elim _ (I.mixed_list_match_n RawMatch.cbor_raw_match SpecRawEverParse.parse_raw_data_item 0 (SZ.v ca_sz) py x.LowParse.PulseParse.Iterator.Type.after l2);
+      Trade.elim _ (I.mixed_list_match_n RawMatch.cbor_raw_match SpecRawEverParse.parse_raw_data_item 0 (SZ.v ca_sz) py (IT.iter_after x) l2);
       // Fold back: original iterator_match
-      rewrite (I.base_mixed_list_match_n RawMatch.cbor_raw_match SpecRawEverParse.parse_raw_data_item 0 (SZ.v cb_sz) py x.LowParse.PulseParse.Iterator.Type.before l1)
-           as (I.base_mixed_list_match RawMatch.cbor_raw_match SpecRawEverParse.parse_raw_data_item py x.LowParse.PulseParse.Iterator.Type.before l1);
-      rewrite (I.mixed_list_match_n RawMatch.cbor_raw_match SpecRawEverParse.parse_raw_data_item 0 (SZ.v ca_sz) py x.LowParse.PulseParse.Iterator.Type.after l2)
-           as (I.mixed_list_match RawMatch.cbor_raw_match SpecRawEverParse.parse_raw_data_item py x.LowParse.PulseParse.Iterator.Type.after l2);
+      rewrite (I.base_mixed_list_match_n RawMatch.cbor_raw_match SpecRawEverParse.parse_raw_data_item 0 (SZ.v cb_sz) py (IT.iter_before x) l1)
+           as (I.base_mixed_list_match RawMatch.cbor_raw_match SpecRawEverParse.parse_raw_data_item py (IT.iter_before x) l1);
+      rewrite (I.mixed_list_match_n RawMatch.cbor_raw_match SpecRawEverParse.parse_raw_data_item 0 (SZ.v ca_sz) py (IT.iter_after x) l2)
+           as (I.mixed_list_match RawMatch.cbor_raw_match SpecRawEverParse.parse_raw_data_item py (IT.iter_after x) l2);
       fold (I.iterator_match RawMatch.cbor_raw_match SpecRawEverParse.parse_raw_data_item py x (Ghost.reveal lr));
       rewrite (I.iterator_match RawMatch.cbor_raw_match SpecRawEverParse.parse_raw_data_item py x (Ghost.reveal lr))
            as (I.iterator_match RawMatch.cbor_raw_match SpecRawEverParse.parse_raw_data_item py x (Aux.det_raw_list z));
@@ -1539,19 +1539,19 @@ fn cbor_det_map_iterator_share (_: unit) : share_t cbor_det_map_iterator_match
     I.base_mixed_list_match
       (fun pm0 e v -> RawMatch.cbor_map_entry_match RawMatch.cbor_raw_match pm0 e v)
       (LowParse.Spec.Combinators.nondep_then SpecRawEverParse.parse_raw_data_item SpecRawEverParse.parse_raw_data_item)
-      pm it.LowParse.PulseParse.Iterator.Type.before l1 **
+      pm (IT.iter_before it) l1 **
     I.mixed_list_match
       (fun pm0 e v -> RawMatch.cbor_map_entry_match RawMatch.cbor_raw_match pm0 e v)
       (LowParse.Spec.Combinators.nondep_then SpecRawEverParse.parse_raw_data_item SpecRawEverParse.parse_raw_data_item)
-      pm it.LowParse.PulseParse.Iterator.Type.after l2);
+      pm (IT.iter_after it) l2);
   I.base_mixed_list_match_share
     (fun pm0 e v -> RawMatch.cbor_map_entry_match RawMatch.cbor_raw_match pm0 e v)
     (LowParse.Spec.Combinators.nondep_then SpecRawEverParse.parse_raw_data_item SpecRawEverParse.parse_raw_data_item)
-    pm it.LowParse.PulseParse.Iterator.Type.before l1 cbor_map_entry_match_share_aux;
+    pm (IT.iter_before it) l1 cbor_map_entry_match_share_aux;
   I.mixed_list_match_share
     (fun pm0 e v -> RawMatch.cbor_map_entry_match RawMatch.cbor_raw_match pm0 e v)
     (LowParse.Spec.Combinators.nondep_then SpecRawEverParse.parse_raw_data_item SpecRawEverParse.parse_raw_data_item)
-    pm it.LowParse.PulseParse.Iterator.Type.after l2 cbor_map_entry_match_share_aux;
+    pm (IT.iter_after it) l2 cbor_map_entry_match_share_aux;
   fold (I.iterator_match
       (fun pm0 e v -> RawMatch.cbor_map_entry_match RawMatch.cbor_raw_match pm0 e v)
       (LowParse.Spec.Combinators.nondep_then SpecRawEverParse.parse_raw_data_item SpecRawEverParse.parse_raw_data_item)
@@ -1602,20 +1602,20 @@ fn cbor_det_map_iterator_is_empty (_: unit) : map_iterator_is_empty_t cbor_det_m
     I.base_mixed_list_match
       (fun pm0 e v -> RawMatch.cbor_map_entry_match RawMatch.cbor_raw_match pm0 e v)
       (LowParse.Spec.Combinators.nondep_then SpecRawEverParse.parse_raw_data_item SpecRawEverParse.parse_raw_data_item)
-      p x.LowParse.PulseParse.Iterator.Type.before l1 **
+      p (IT.iter_before x) l1 **
     I.mixed_list_match
       (fun pm0 e v -> RawMatch.cbor_map_entry_match RawMatch.cbor_raw_match pm0 e v)
       (LowParse.Spec.Combinators.nondep_then SpecRawEverParse.parse_raw_data_item SpecRawEverParse.parse_raw_data_item)
-      p x.LowParse.PulseParse.Iterator.Type.after l2);
+      p (IT.iter_after x) l2);
   I.base_mixed_list_match_length
     (fun pm0 e v -> RawMatch.cbor_map_entry_match RawMatch.cbor_raw_match pm0 e v)
     (LowParse.Spec.Combinators.nondep_then SpecRawEverParse.parse_raw_data_item SpecRawEverParse.parse_raw_data_item)
-    p x.LowParse.PulseParse.Iterator.Type.before l1;
+    p (IT.iter_before x) l1;
   I.mixed_list_match_length
     (fun pm0 e v -> RawMatch.cbor_map_entry_match RawMatch.cbor_raw_match pm0 e v)
     (LowParse.Spec.Combinators.nondep_then SpecRawEverParse.parse_raw_data_item SpecRawEverParse.parse_raw_data_item)
-    p x.LowParse.PulseParse.Iterator.Type.after l2;
-  let len_before = IT.base_mixed_list_length x.LowParse.PulseParse.Iterator.Type.before;
+    p (IT.iter_after x) l2;
+  let len_before = IT.base_mixed_list_length (IT.iter_before x);
   Aux.length_det_raw_map_entries y;
   let res = (len_before = 0sz);
   fold (I.iterator_match
@@ -1670,28 +1670,28 @@ fn cbor_det_map_iterator_gather (_: unit) : gather_t cbor_det_map_iterator_match
     I.base_mixed_list_match
       (fun pm0 e v -> RawMatch.cbor_map_entry_match RawMatch.cbor_raw_match pm0 e v)
       (LowParse.Spec.Combinators.nondep_then SpecRawEverParse.parse_raw_data_item SpecRawEverParse.parse_raw_data_item)
-      pm it.LowParse.PulseParse.Iterator.Type.before l1 **
+      pm (IT.iter_before it) l1 **
     I.mixed_list_match
       (fun pm0 e v -> RawMatch.cbor_map_entry_match RawMatch.cbor_raw_match pm0 e v)
       (LowParse.Spec.Combinators.nondep_then SpecRawEverParse.parse_raw_data_item SpecRawEverParse.parse_raw_data_item)
-      pm it.LowParse.PulseParse.Iterator.Type.after l2);
+      pm (IT.iter_after it) l2);
   with l1' l2' . assert (
     I.base_mixed_list_match
       (fun pm0 e v -> RawMatch.cbor_map_entry_match RawMatch.cbor_raw_match pm0 e v)
       (LowParse.Spec.Combinators.nondep_then SpecRawEverParse.parse_raw_data_item SpecRawEverParse.parse_raw_data_item)
-      pm' it.LowParse.PulseParse.Iterator.Type.before l1' **
+      pm' (IT.iter_before it) l1' **
     I.mixed_list_match
       (fun pm0 e v -> RawMatch.cbor_map_entry_match RawMatch.cbor_raw_match pm0 e v)
       (LowParse.Spec.Combinators.nondep_then SpecRawEverParse.parse_raw_data_item SpecRawEverParse.parse_raw_data_item)
-      pm' it.LowParse.PulseParse.Iterator.Type.after l2');
+      pm' (IT.iter_after it) l2');
   I.base_mixed_list_match_gather
     (fun pm0 e v -> RawMatch.cbor_map_entry_match RawMatch.cbor_raw_match pm0 e v)
     (LowParse.Spec.Combinators.nondep_then SpecRawEverParse.parse_raw_data_item SpecRawEverParse.parse_raw_data_item)
-    pm pm' it.LowParse.PulseParse.Iterator.Type.before l1 l1' cbor_map_entry_match_gather_aux;
+    pm pm' (IT.iter_before it) l1 l1' cbor_map_entry_match_gather_aux;
   I.mixed_list_match_gather
     (fun pm0 e v -> RawMatch.cbor_map_entry_match RawMatch.cbor_raw_match pm0 e v)
     (LowParse.Spec.Combinators.nondep_then SpecRawEverParse.parse_raw_data_item SpecRawEverParse.parse_raw_data_item)
-    pm pm' it.LowParse.PulseParse.Iterator.Type.after l2 l2' cbor_map_entry_match_gather_aux;
+    pm pm' (IT.iter_after it) l2 l2' cbor_map_entry_match_gather_aux;
   List.Tot.append_injective l1 l1' l2 l2';
   fold (I.iterator_match
       (fun pm0 e v -> RawMatch.cbor_map_entry_match RawMatch.cbor_raw_match pm0 e v)
