src/lowparse/pulse/LowParse.PulseParse.Iterator.Type.fst
@@ -36,10 +36,27 @@ type mixed_list ([@@@strictly_positive] t: Type) =
   mixed_list t
 
 noeq
-type iterator ([@@@strictly_positive] t: Type) = {
-  before: base_mixed_list t;
-  after: mixed_list t
-}
+type iterator ([@@@strictly_positive] t: Type) =
+| IBase: (before: base_mixed_list t) -> iterator t
+| IPair: (before: base_mixed_list t) -> (after: mixed_list t) -> iterator t
+
+inline_for_extraction
+let iter_before
+  (#t: Type)
+  (i: iterator t)
+: Tot (base_mixed_list t)
+= match i with
+  | IBase bi -> bi
+  | IPair bi _ -> bi
+
+inline_for_extraction
+let iter_after
+  (#t: Type)
+  (i: iterator t)
+: Tot (mixed_list t)
+= match i with
+  | IBase _ -> Base (Empty #t)
+  | IPair _ ml -> ml
 
 let base_mixed_list_length
   (#t: Type)
